end of day 16/06/19

formal/Contexts.thy
@@ -7,614 +7,84 @@ transitions with register update functions.
 
 theory Contexts
   imports
-    EFSM GExp CExp
+    EFSM GExp
 begin
 
-type_synonym "context" = "aexp \<Rightarrow> cexp fset"
+definition can_take :: "transition \<Rightarrow> inputs \<Rightarrow> registers \<Rightarrow> bool" where
+  "can_take t i r = apply_guards (Guard t) (join_ir i r)"
 
-(*Decided to keep this as Bc True in order to oversimplify relatiy - strictly this should be
-"Not Undef" for "has a value but we don't know what it is but this doesn't allow for
-oversimplification*)
-abbreviation empty :: "context" ("\<lbrakk>\<rbrakk>") where
-  "empty \<equiv> (\<lambda>x. case x of
-    (V v) \<Rightarrow> (case v of R n \<Rightarrow> {|Undef|} | I n \<Rightarrow> {|Bc True|}) |
-    _ \<Rightarrow> {|Bc True|}
-  )"
-syntax
-  "_updbind" :: "'a \<Rightarrow> 'a \<Rightarrow> updbind" ("(2_ \<mapsto>/ _)")
-  "_Context" :: "updbinds \<Rightarrow> 'a"      ("\<lbrakk>_\<rbrakk>")
-translations
-  "_Update f (_updbinds b bs)" \<rightleftharpoons> "_Update (_Update f b) bs"
-  "_Context ms" == "_Update \<lbrakk>\<rbrakk> ms"
-  "_Context (_updbinds b bs)" \<rightleftharpoons> "_Update (_Context b) bs"
+definition medial :: "datastate \<Rightarrow> transition \<Rightarrow> bool" where
+  "medial c t = apply_guards (Guard t) c"
 
-lemma empty_register: "\<lbrakk>\<rbrakk> (V (R r)) = {|Undef|}"
-  by (simp)
+definition strip_inputs :: "datastate \<Rightarrow> registers" where
+  "strip_inputs d = (\<lambda>r. d (R r))"
 
-lemma empty_input: "\<lbrakk>\<rbrakk> (V (I i)) = {|Bc True|}"
-  by (simp)
+definition posterior :: "transition \<Rightarrow> datastate \<Rightarrow> registers option" where
+  "posterior t d = (if medial d t then Some (apply_updates (Updates t) d (strip_inputs d)) else None)"
 
-lemma consistent_empty_fball: "fBall (\<lbrakk>\<rbrakk> r) (\<lambda>c. cval c r Map.empty = true)"
-  apply (cases r)
-     apply (simp add: cval_true)
-    apply (case_tac x2)
-     apply (simp add: cval_true)
-    apply (simp add: cval_def gval.simps ValueEq_def)
-  using cval_true by auto
+definition subsumes :: "transition \<Rightarrow> datastate \<Rightarrow> transition \<Rightarrow> bool" where
+  "subsumes t2 c t1 = (medial c t1 \<longrightarrow> medial c t2 \<and>
+                       medial c t1 \<longrightarrow> apply_outputs (Outputs t1) c = apply_outputs (Outputs t2) c \<and>
+                       (\<exists>p1 p2. posterior t2 c = Some p1 \<and> posterior t2 c = Some p2 \<longrightarrow> (\<forall>P. P p1 \<longrightarrow> P p2)) \<and> 
+                       (\<exists>p1 p2. posterior t2 c = Some p1 \<longrightarrow> posterior t2 c = Some p2))"
 
-lemma empty_not_false[simp]: "{|Bc False|} \<noteq> \<lbrakk>\<rbrakk> i"
-proof (induct i)
-case (L x)
-then show ?case by simp
-next
-  case (V x)
-  then show ?case
-    apply (case_tac x)
-    by simp_all
-next
-  case (Plus i1 i2)
-  then show ?case
-    by simp
-next
-  case (Minus i1 i2)
-  then show ?case
-    by simp
-qed
-
-lemma empty_variable_constraints: "\<lbrakk>\<rbrakk> (V (R ri)) = {|Undef|} \<and> \<lbrakk>\<rbrakk> (V (I i)) = {|Bc True|}"
-  by simp
-
-fun get :: "context \<Rightarrow> aexp \<Rightarrow> cexp fset" where
-  "get c (L n) = {|Eq n|}" |
-  "get c (V v) = c (V v)" |
-  "get c (Plus v va) = (c (Plus v va)) |\<union>| (c (Plus va v))" |
-  "get c (Minus v va) = (c (Minus v va))"
-
-fun update :: "context \<Rightarrow> aexp \<Rightarrow> cexp fset \<Rightarrow> context" where
-  "update c (L n) _ = c" |
-  "update c k v = (\<lambda>r. if r=k then v else c r)"
-
-definition conjoin :: "cexp fset \<Rightarrow> cexp" where
-  "conjoin f = foldr And (sorted_list_of_fset f) (Bc True)"
-
-definition consistent :: "context \<Rightarrow> bool" where (* Is there a variable evaluation which can satisfy all of the context? *)
-  "consistent c \<equiv> \<exists>s. \<forall>r. fBall (c r) (\<lambda>c. (cval c r s = true))"
-
-lemma subset_consistency: "\<forall>r. c' r |\<subseteq>| c r \<Longrightarrow> consistent c \<Longrightarrow> consistent c'"
-  apply (simp add: consistent_def)
-  apply clarify
-  apply (rule_tac x=s in exI)
-  by auto
-
-lemma possible_false_not_consistent: "\<exists>r. c r = {|Bc False|} \<Longrightarrow> \<not> consistent c"
-  apply (simp add: consistent_def conjoin_def)
-  apply clarify
-  apply (rule_tac x=r in exI)
-  by (simp add: sorted_list_of_fset_def cval_And cval_false cval_true)
-
-lemma inconsistent_false: "\<not>consistent (\<lambda>i. {|Bc False|})"
-  using possible_false_not_consistent
-  by simp
-
-lemma consistent_empty_1: "empty r = {|Undef|} \<or> empty r = {|Bc True|}"
-  apply (cases r)
-  prefer 2
-    apply (case_tac x2)
-  by simp_all
-
-theorem consistent_empty_2: "(\<forall>r. c r = {|Bc True|}) \<longrightarrow> consistent c"
-  apply (simp add: consistent_def conjoin_def sorted_list_of_fset_def)
-  by (simp add: cval_And cval_true)
-
-lemma consistent_empty_4: "\<lbrakk>\<rbrakk> r = {|Undef|} \<or> gval (cexp2gexp r (conjoin (\<lbrakk>\<rbrakk> r))) c = true"
-  apply (case_tac r)
-     apply (simp add: consistent_def conjoin_def sorted_list_of_fset_def maybe_double_negation)
-     apply (simp add: gval_gAnd gval.simps(1))
-    apply (case_tac x2)
-     apply (simp add: conjoin_def sorted_list_of_fset_def gval_gAnd gval.simps(1))
-    apply (simp add: conjoin_def)
-   apply (simp add: conjoin_def sorted_list_of_fset_def gval_gAnd gval.simps(1))
-  by (simp add: conjoin_def sorted_list_of_fset_def gval_gAnd gval.simps(1))
-
-lemma consistent_empty [simp]: "consistent empty"
-  apply (simp add: consistent_def cval_def)
-  apply (rule_tac x="<>" in exI)
-  apply clarify
-  apply (case_tac r)
-     apply (simp add: conjoin_def sorted_list_of_fset_def gval_gAnd gval.simps(1))
-    apply (case_tac x2)
-  by (simp_all add: conjoin_def sorted_list_of_fset_def gval_gAnd gval.simps ValueEq_def)
-
-lemma cexp2gexp_double_neg: "gexp_equiv (cexp2gexp r (Not (Not x))) (cexp2gexp r x)"
-  apply (simp add: gexp_equiv_def gval_gAnd)
-  by (simp add: maybe_and_idempotent)
-
-lemma gval_cexp2gexp_double_neg: "gval (cexp2gexp r (Not (Not x))) s = gval (cexp2gexp r x) s"
-  using cexp2gexp_double_neg gexp_equiv_def by blast
-
-fun make_gt :: "cexp \<Rightarrow> cexp" where
-  "make_gt (Bc b) = Bc b" |
-  "make_gt Undef = Undef" |
-  "make_gt (Eq v) = Gt v" |
-  "make_gt (Lt v) = Bc True" |
-  "make_gt (Gt s) = Gt s" |
-  "make_gt (Not v) = Not (make_gt v)" |
-  "make_gt (And v va) = And (make_gt v) (make_gt va)"
-
-lemma make_gt_twice: "make_gt (make_gt x) = make_gt x"
-  apply (induct x)
-  by auto
-
-lemma cval_make_gt_not: "cval (make_gt (not x)) r s = maybe_not (cval (make_gt x) r s)"
-proof(induct x)
-case Undef
-  then show ?case
-    by (simp add: cval_Not)
-next
-  case (Bc x)
-  then show ?case
-    apply simp
-    by (metis cval_not not.simps(1))
-next
-  case (Eq x)
-  then show ?case
-    by (simp add: cval_Not)
-next
-  case (Lt x)
-  then show ?case
-    by (simp add: cval_Not cval_false cval_true)
-next
-  case (Gt x)
-  then show ?case
-    by (simp add: cval_Not)
-next
-  case (Not x)
-  then show ?case
-    by (simp add: cval_Not maybe_double_negation)
-next
-  case (And x1 x2)
-  then show ?case
-    apply simp
-    by (simp only: cval_And cval_Not cval_and)
-qed
-
-fun make_lt :: "cexp \<Rightarrow> cexp" where
-  "make_lt (Bc b) = Bc b" |
-  "make_lt Undef = Undef" |
-  "make_lt (Eq v) = Lt v" |
-  "make_lt (Lt v) = Lt v" |
-  "make_lt (Gt v) = Bc True" |
-  "make_lt (Not v) = Not (make_lt v)" |
-  "make_lt (And v va) = And (make_lt v) (make_lt va)"
-
-lemma make_lt_twice: "make_lt (make_lt x) = make_lt x"
-  apply(induct x)
-  by auto
-
-fun guard2pairs :: "context \<Rightarrow> gexp \<Rightarrow> (aexp \<times> cexp fset) list" where
-  "guard2pairs a (gexp.Bc True) = []" |
-  "guard2pairs a (gexp.Bc False) = [(L (Num 0), {|Bc False|})]" |
-
-  "guard2pairs a (gexp.Null v) = [(v, {|Undef|})]" |
-
-  "guard2pairs a (gexp.Eq v (L n)) = [(v, {|Eq n|})]" |
-  "guard2pairs a (gexp.Eq (L n) v) = [(v, {|Eq n|})]" |
-  "guard2pairs a (gexp.Eq (Plus a1 a2) (Plus a4 a3)) = [((Plus a1 a2), (get a (Plus a2 a1)) |\<union>| (get a (Plus a3 a4))),
-                                                        ((Plus a2 a1), (get a (Plus a1 a2)) |\<union>| (get a (Plus a3 a4))),
-                                                        ((Plus a3 a4), (get a (Plus a4 a3)) |\<union>| (get a (Plus a1 a2))),
-                                                        ((Plus a4 a3), (get a (Plus a3 a4)) |\<union>| (get a (Plus a1 a2)))]" |
-  "guard2pairs a (gexp.Eq (Plus a1 a2) v) = [((Plus a1 a2), (get a v) |\<union>| (get a (Plus a1 a2))),
-                                             ((Plus a2 a1), (get a v) |\<union>| (get a (Plus a2 a1))),
-                                             (v, get a (Plus a1 a2))]" |
-  "guard2pairs a (gexp.Eq v (Plus a1 a2)) = [((Plus a1 a2), (get a v) |\<union>| (get a (Plus a1 a2))),
-                                             ((Plus a2 a1), (get a v) |\<union>| (get a (Plus a2 a1))),
-                                             (v, get a (Plus a1 a2))]" |
-  "guard2pairs a (gexp.Eq v va) = [(v, get a va), (va, get a v)]" |
-
-  "guard2pairs a (gexp.Gt (L v) va) = (if L v = va then [(L (Num 0), {|Bc False|})] else [(va, {|Lt v|})])" |
-  "guard2pairs a (gexp.Gt va (L v)) = (if L v = va then [(L (Num 0), {|Bc False|})] else [(va, {|Gt v|})])" |
-  "guard2pairs a (gexp.Gt v vb) = (if v = vb then
-                                     [(L (Num 0), {|Bc False|})]
-                                   else
-                                     [(v, fimage make_gt (get a vb))]
-                                  )" |
-
-  "guard2pairs a (Nor v va) = (map (\<lambda>(x, y). (x, fimage not y)) ((guard2pairs a v) @ (guard2pairs a va)))"
-
-definition pairs2context :: "(aexp \<times> cexp fset) list \<Rightarrow> context" where
-  "pairs2context l = (\<lambda>r. fold funion (map snd (filter (\<lambda>(a, _). a = r) l)) {||})"
-
-lemma pairs2context_empty: "pairs2context [] x = {||}"
-  by (simp add: pairs2context_def)
-
-lemma pairs2context_append: "pairs2context (x @ y) ra = pairs2context x ra |\<union>| pairs2context y ra"
-  apply (simp only: pairs2context_def)
-  by (metis ffUnion_funion_distrib filter_append fold_union_ffUnion fset_of_list_append map_append map_eq_map_tailrec)
-
-lemma pairs2context_cons: "pairs2context (x # y) ra = pairs2context [x] ra |\<union>| pairs2context y ra"
-  by (metis append_Cons append_self_conv2 pairs2context_append)
-
-definition medial :: "context \<Rightarrow> gexp list \<Rightarrow> context" where
- "medial c G = (\<lambda>r. (c r) |\<union>| pairs2context (List.maps (guard2pairs c) G) r)"
-
-lemma medial_cons: "medial c (a # G) ra = medial c [a] ra |\<union>| medial c G ra"
-  apply (simp only: medial_def)
-  by (simp add: inf_sup_aci(5) inf_sup_aci(7) maps_simps(1) maps_simps(2) pairs2context_append)
-
-lemma List_maps_append:  "List.maps f (a@g) = (List.maps f a)@(List.maps f g)"
-  by (simp add: List.maps_def)
-
-lemma medial_append: "medial c (a @ G) ra = medial c a ra |\<union>| medial c G ra"
-  apply (simp only: medial_def List_maps_append pairs2context_append)
-  by auto
-
-lemma medial_append_commutative: "medial c (g1 @ g2) = medial c (g2 @ g1)"
-  unfolding medial_append
-  by auto
-
-lemma medial_self_append: "medial c (g @ g) = medial c g"
-  apply (rule ext)
-  by (simp add: medial_append)
-
-lemma medial_cons_subset: "medial c G ra |\<subseteq>| medial c (a # G) ra"
-  apply (simp add: medial_def)
-  apply (simp only: maps_simps(1))
-  apply (simp only: pairs2context_append)
-  by auto
-
-lemma equality_guard_gives_equality_constraint: 
-  "(\<exists> v. gexp.Eq (V (I i)) (L v) \<in> set G) \<Longrightarrow>
-    \<exists>v. (Eq v) |\<in>| medial c G (V (I i))"
-proof(induct G)
-  case Nil
-  then show ?case by simp
-next
-  case (Cons a G)
-  then show ?case
-    apply (simp add: medial_def)
-    apply clarify
-    apply (case_tac "\<exists>v. cexp.Eq v |\<in>| c (V (I i))")
-     apply auto[1]
-    apply simp
-    apply (case_tac "a = gexp.Eq (V (I i)) (L v)")
-     apply (simp add: pairs2context_def List.maps_def)
-     apply (rule_tac x=v in exI)
-     apply (simp add: fold_invariant)
-    apply simp
-    using medial_cons medial_def by fastforce
-qed
-
-lemma medial_filter: "medial c (filter f G) ra |\<subseteq>| medial c G ra"
-proof(induct G)
-  case Nil
-  then show ?case by simp
-next
-  have aux1: "\<forall>a f G ra c. medial c (a # filter f G) ra = medial c [a] ra |\<union>| medial c (filter f G) ra"
-    using medial_cons by blast
-  case (Cons a G)
-  then show ?case
-    apply simp
-    apply (case_tac "f a")
-     apply simp
-     defer
-    apply simp
-    using medial_cons_subset apply blast
-    apply (simp only: aux1)
-  proof -
-    assume "medial c (filter f G) ra |\<subseteq>| medial c G ra"
-    then have "medial c (a # G) ra = medial c [a] ra |\<union>| (medial c G ra |\<union>| medial c (filter f G) ra |\<union>| medial c (filter f G) ra)"
-      using medial_cons by blast
-    then show "medial c [a] ra |\<union>| medial c (filter f G) ra |\<subseteq>| medial c (a # G) ra"
-      by blast
-  qed
-qed
-
-lemma medial_empty: "medial c [] = c"
-  by (simp add: medial_def pairs2context_def List.maps_def)
-
-lemma anterior_subset_medial: "c r |\<subseteq>| (medial c G r)"
-    by (simp add: medial_def pairs2context_def)
-
-fun apply_update :: "context \<Rightarrow> context \<Rightarrow> update_function \<Rightarrow> context" where
-  "apply_update l c (v, (L n)) = update c (V v) {|(Eq n)|}" |
-  "apply_update l c (v, V vb) = update c (V v) (l (V vb))" |
-  "apply_update l c (v, Plus vb vc) = update c (V v) (fimage (\<lambda>(a, b). compose_plus a b) ((get l vb) |\<times>| (get l vc)))" |
-  "apply_update l c (v, Minus vb vc) = update c (V v) (fimage (\<lambda>(a, b). compose_minus a b) ((get l vb) |\<times>| (get l vc)))"
-
-lemma not_updated_stays_the_same: "aa \<noteq> r \<Longrightarrow> apply_update m a (aa, b) (V r) = a (V r)"
-proof(induct b)
-  case (L x)
-  then show ?case by simp
-next
-  case (V x)
-  then show ?case
-    by simp
-next
-  case (Plus b1 b2)
-  then show ?case
-    by simp
-next
-  case (Minus b1 b2)
-  then show ?case
-    by simp
-qed
-
-primrec apply_updates :: "context \<Rightarrow> context \<Rightarrow> update_function list \<Rightarrow> context" where
-  "apply_updates _ c [] = c" |
-  "apply_updates l c (h#t) = (apply_update l (apply_updates l c t) h)"
-
-lemma not_updated_stays_the_same_2: "filter (\<lambda>(r', u). r' = r) u = [] \<Longrightarrow> 
-       apply_updates m c u (V r) = c (V r)"
-proof(induct u)
-  case Nil
-  then show ?case by simp
-next
-  case (Cons a u)
-  then show ?case
-    apply (case_tac a)
-    apply simp
-    apply (case_tac "aa = r")
-     apply simp
-    by (simp add: not_updated_stays_the_same)
-qed
-
-lemma updated_variable_value: "(r, (V v)) \<in> set u \<Longrightarrow>
-       length (filter (\<lambda>(r', u). r' = r) u) = 1 \<Longrightarrow>
-       apply_updates m c u (V r) = m (V v)"
-proof(induct u)
-  case Nil
-  then show ?case
-    by simp
-next
-  case (Cons a u)
-  then show ?case
-    apply simp
-    apply (case_tac "a = (r, V v)")
-     apply simp
-    apply simp
-    apply (cases a)
-    apply clarify
-    apply (case_tac "aa = r")
-     apply simp
-     apply (metis (mono_tags, lifting) case_prodI filter_empty_conv)
-    by (simp add: not_updated_stays_the_same)
-qed
-
-definition can_take :: "transition \<Rightarrow> context \<Rightarrow> bool" where
-  "can_take t c \<equiv> consistent (medial c (Guard t))"
-
-lemma can_take_no_guards: "\<forall> c. (Contexts.consistent c \<and> (Guard t) = []) \<longrightarrow> Contexts.can_take t c"
-  by (simp add: consistent_def Contexts.can_take_def medial_def pairs2context_def List.maps_def)
-
-fun constrains_an_input :: "aexp \<Rightarrow> bool" where
-  "constrains_an_input (L v) = False" |
-  "constrains_an_input (V (R x)) = False" |
-  "constrains_an_input (V (I x)) = True" |
-  "constrains_an_input (Plus v va) = (constrains_an_input v \<or> constrains_an_input va)" |
-  "constrains_an_input (Minus v va) = (constrains_an_input v \<or> constrains_an_input va)"
-
-definition remove_obsolete_constraints :: "context \<Rightarrow> vname fset \<Rightarrow> context" where
-  "remove_obsolete_constraints c vs = (\<lambda>a. if \<exists>n. aexp_constrains a (V (I n)) \<or> fBex vs (\<lambda>x. aexp_constrains (V x) a \<and> a \<noteq> (V x)) then \<lbrakk>\<rbrakk> a else c a)"
-
-lemma consistent_c_consistent_remove_obsolete_constraints: "consistent c \<Longrightarrow> consistent (remove_obsolete_constraints c Any)"
-  apply (simp add: remove_obsolete_constraints_def consistent_def)
-  apply clarify
-  apply (rule_tac x=s in exI)
-  apply clarify
-  apply (case_tac r)
-     apply simp
-  apply (case_tac x2)
-  using cval_true by auto
-
-lemma empty_inputs_are_true: "constrains_an_input x \<Longrightarrow> \<lbrakk>\<rbrakk> x = {|Bc True|}"
-  apply (case_tac x)
-     apply simp
-    apply (case_tac x2)
-  by auto
-
-lemma cval_empty_inputs: "constrains_an_input r \<longrightarrow> cval (conjoin (\<lbrakk>\<rbrakk> r)) r ia = true"
-proof(induct r)
-case (L x)
-  then show ?case by simp
-next
-  case (V x)
-  then show ?case
-    apply (cases x)
-     apply (simp add: conjoin_def sorted_list_of_fset_def)
-     apply (simp only: cval_And maybe_and_true cval_true)
-    by simp
-next
-  case (Plus r1 r2)
-  then show ?case
-    apply (simp add: conjoin_def sorted_list_of_fset_def)
-    apply (simp only: cval_And maybe_and_true cval_true)
-    by simp
-next
-  case (Minus r1 r2)
-  then show ?case
-    apply (simp add: conjoin_def sorted_list_of_fset_def)
-    apply (simp only: cval_And maybe_and_true cval_true)
-    by simp
-qed
-
-lemma remove_input_constraints_empty[simp]: "remove_obsolete_constraints \<lbrakk>\<rbrakk> s = \<lbrakk>\<rbrakk>"
-  by (simp add: remove_obsolete_constraints_def)
-
-definition posterior_separate :: "context \<Rightarrow> gexp list \<Rightarrow> update_function list \<Rightarrow> context" where (* Corresponds to Algorithm 1 in Foster et. al. *)
-  "posterior_separate c g u = (let c' = (medial c g) in (if consistent c' then remove_obsolete_constraints (apply_updates c' c u) (fset_of_list (map fst u)) else (\<lambda>i. {|Bc False|})))"
-
-lemma posterior_separate_append_self: "posterior_separate c (g @ g) = posterior_separate c g"
-  apply (rule ext)
-  by (simp add: posterior_separate_def Let_def medial_self_append)
-
-definition posterior :: "context \<Rightarrow> transition \<Rightarrow> context" where
-  "posterior c t = posterior_separate c (Guard t) (Updates t)"
-
-lemma posterior_consistent_medial: "medial c (Guard t) = c' \<Longrightarrow> consistent c' \<Longrightarrow> remove_obsolete_constraints (apply_updates c' c (Updates t)) (fst |`| fset_of_list (Updates t)) = p \<Longrightarrow> posterior c t = p"
-  by (simp add: posterior_def posterior_separate_def)
-
-primrec posterior_n :: "nat \<Rightarrow> transition \<Rightarrow> context \<Rightarrow> context" where (* Apply a given transition to a given context n times - good for reflexive transitions*)
-  "posterior_n 0 _ c = c " |
-  "posterior_n (Suc m) t c = posterior_n m t (posterior c t)"
-
-primrec posterior_sequence :: "context \<Rightarrow> transition_matrix \<Rightarrow> nat \<Rightarrow> datastate \<Rightarrow> trace \<Rightarrow> context" where
-  "posterior_sequence c _ _ _ [] = c" |
-  "posterior_sequence c e s r (h#t) =
-    (case (step e s r (fst h) (snd h)) of
-      (Some (transition, s', outputs, r')) \<Rightarrow> (posterior_sequence (posterior c transition) e s' r' t) |
-      _ \<Rightarrow> c
-    )"
-
-definition datastate2context :: "datastate \<Rightarrow> context" where
-  "datastate2context d = (\<lambda>x. case x of V r \<Rightarrow> (case d r of None \<Rightarrow> {|Undef|} | Some v \<Rightarrow> {|Eq v|}) | _ \<Rightarrow> \<lbrakk>\<rbrakk> x)"
-
-definition satisfies_context :: "datastate \<Rightarrow> context \<Rightarrow> bool" where
-  "satisfies_context d c = consistent (\<lambda>x. (datastate2context d x) |\<union>| c x)"
-
-lemma satisfactory_registers: "c (V (R r)) = {|cexp.Eq v|} \<Longrightarrow>
-       satisfies_context ra c \<Longrightarrow>
-       ra (R r) = Some v"
-proof-
-  assume premise1: "c (V (R r)) = {|cexp.Eq v|}"
-  assume premise2: "satisfies_context ra c"
-  have contra: "c (V (R r)) = {|cexp.Eq v|} \<Longrightarrow>
-                ra (R r) \<noteq> Some v \<Longrightarrow>
-                \<not>satisfies_context ra c"
-    apply (simp add: satisfies_context_def datastate2context_def consistent_def)
-    apply clarify
-    apply (rule_tac x="V (R r)" in exI)
-    apply (simp add: cval_def)
-    apply (case_tac "ra (R r)")
-    using gval.simps ValueEq_def
-    by auto
-  show ?thesis
-    using premise1 premise2 contra by auto
-qed
-
-lemma cval_undef_empty: "cval Undef (V x) <> = true"
-  by (simp add: cval_def gval.simps ValueEq_def)
-
-lemma satisfies_context_empty: "satisfies_context <> \<lbrakk>\<rbrakk> \<and> satisfies_context Map.empty \<lbrakk>\<rbrakk>"
-  apply (simp add: satisfies_context_def datastate2context_def consistent_def)
-  apply (rule_tac x="<>" in exI)
-  apply clarify
-  apply (case_tac r)
-     apply (simp add: cval_true)
-    apply (case_tac x2)
-     apply (case_tac "x=Bc True")
-  by (simp_all add: cval_true cval_def gval.simps ValueEq_def)
-
-(* Does t2 subsume t1? *)
-definition subsumes :: "transition \<Rightarrow> context \<Rightarrow> transition \<Rightarrow> bool" ("_\<^sub>_\<sqsupseteq>_" 60) where (* Corresponds to Algorithm 2 in Foster et. al. *)
-  "subsumes t2 c t1 \<equiv> Label t1 = Label t2 \<and> Arity t1 = Arity t2 \<and> length (Outputs t1) = length (Outputs t2) \<and>
-                      (\<forall>r i. fBall (medial c (Guard t1) r) (\<lambda>c. cval c r i = true) \<longrightarrow> fBall (medial c (Guard t2) r) (\<lambda>c. cval c r i = true)) \<and>
-                      (\<forall> i r. satisfies_context r c \<longrightarrow> apply_guards (Guard t1) (join_ir i r) \<longrightarrow> apply_outputs (Outputs t1) (join_ir i r) = apply_outputs (Outputs t2) (join_ir i r)) \<and>
-                      (\<exists> i r. apply_outputs (Outputs t1) (join_ir i r) = apply_outputs (Outputs t2) (join_ir i r)) \<and>
-                      (\<forall>r i. fBall (posterior_separate c (Guard t1@Guard t2) (Updates t2) r) (\<lambda>c. cval c r i = true) \<longrightarrow> fBall (posterior c t1 r) (\<lambda>c. cval c r i = true) \<or> (posterior c t1 r) = {|Undef|}) \<and>
-                      (consistent (posterior c t1) \<longrightarrow> consistent (posterior c t2))"
-
-lemma output_subsumption_violation: "\<not> (\<forall> i r. satisfies_context r c \<longrightarrow> apply_guards (Guard t1) (join_ir i r) \<longrightarrow> apply_outputs (Outputs t1) (join_ir i r) = apply_outputs (Outputs t2) (join_ir i r)) \<Longrightarrow>
-      \<not> subsumes t2 c t1"
-  by (simp add: subsumes_def)
-
-lemma medial_subsumption_violation: "\<not> (\<forall>r i. fBall (medial c (Guard t1) r) (\<lambda>c. cval c r i = true) \<longrightarrow> fBall (medial c (Guard t2) r) (\<lambda>c. cval c r i = true)) \<Longrightarrow>
-\<not> subsumes t2 c t1"
-  by (simp add: subsumes_def)
-
-lemma update_subsumption_violation: "\<not> (\<forall>r i. fBall (posterior_separate c (Guard t1@Guard t2) (Updates t2) r) (\<lambda>c. cval c r i = true) \<longrightarrow> fBall (posterior c t1 r) (\<lambda>c. cval c r i = true) \<or> (posterior c t1 r) = {|Undef|}) \<Longrightarrow>
-      \<not> subsumes t2 c t1"
-  by (simp add: subsumes_def)
-
-lemma outputs_never_equal: "\<not>(\<exists> i r. apply_outputs (Outputs t1) (join_ir i r) = apply_outputs (Outputs t2) (join_ir i r)) \<Longrightarrow>
-\<not> subsumes t2 c t1"
-  by (simp add: subsumes_def)
-
-lemma subsumption: "Label t1 = Label t2 \<and>
-                    Arity t1 = Arity t2 \<and>
-                    length (Outputs t1) = length (Outputs t2) \<Longrightarrow>
-                    (\<forall>r i. fBall (medial c (Guard t1) r) (\<lambda>c. cval c r i = true) \<longrightarrow> fBall (medial c (Guard t2) r) (\<lambda>c. cval c r i = true)) \<Longrightarrow>
-                    (\<forall> i r. satisfies_context r c \<longrightarrow> apply_guards (Guard t1) (join_ir i r) \<longrightarrow> apply_outputs (Outputs t1) (join_ir i r) = apply_outputs (Outputs t2) (join_ir i r)) \<Longrightarrow>
-                    (\<exists> i r. apply_outputs (Outputs t1) (join_ir i r) = apply_outputs (Outputs t2) (join_ir i r)) \<Longrightarrow>
-                    (\<forall>r i. fBall (posterior_separate c (Guard t1@Guard t2) (Updates t2) r) (\<lambda>c. cval c r i = true) \<longrightarrow> fBall (posterior c t1 r) (\<lambda>c. cval c r i = true) \<or> (posterior c t1 r) = {|Undef|}) \<Longrightarrow>
-                    (consistent (posterior c t1) \<longrightarrow> consistent (posterior c t2)) \<Longrightarrow>
-                    subsumes t2 c t1"
-  by (simp add: subsumes_def)
-
-definition anterior_context :: "transition_matrix \<Rightarrow> trace \<Rightarrow> context" where
- "anterior_context e t = posterior_sequence \<lbrakk>\<rbrakk> e 0 <> t"
-
-lemma gexp_equiv_cexp_not_true:  "gexp_equiv (cexp2gexp a (Not (Bc True))) (gexp.Bc False)"
-  by (simp add: gexp_equiv_def gval.simps)
-
-lemma gexp_equiv_cexp_not_false:  "gexp_equiv (cexp2gexp a (Not (Bc False))) (gexp.Bc True)"
-  by (simp add: gexp_equiv_def gval.simps)
-
-lemma geq_to_ge: "Geq x = c r \<Longrightarrow> (cexp2gexp r (c r)) = Ge r (L x)"
-  by (metis cexp2gexp.simps(3) cexp2gexp.simps(6))
-
-lemma leq_to_le: "Leq x = c r \<Longrightarrow> (cexp2gexp r (c r)) = Le r (L x)"
-  by (metis cexp2gexp.simps(4) cexp2gexp.simps(6))
-
-lemma lt_to_lt: "Lt x = c r \<Longrightarrow> (cexp2gexp r (c r)) = gexp.Gt (L x) r"
-  by (metis cexp2gexp.simps(3))
-
-lemma gt_to_gt: "Gt x = c r \<Longrightarrow> (cexp2gexp r (c r)) = gexp.Gt r (L x)"
-  by (metis cexp2gexp.simps(4))
-
-lemma satisfiable_double_neg: "satisfiable (cexp.Not (cexp.Not x)) = satisfiable x"
-  by (simp add: satisfiable_def cval_double_negation)
-
-lemma gval_empty_r_neq_none[simp]: "gval (cexp2gexp r (conjoin (\<lbrakk>\<rbrakk> r))) s \<noteq> invalid"
-  apply (case_tac r)
-     apply (simp add: conjoin_def sorted_list_of_fset_def maybe_double_negation gval.simps)
-    apply (case_tac x2)
-  by (simp_all add: conjoin_def sorted_list_of_fset_def gval_gAnd gval.simps ValueEq_def)
-
-lemma constrains_an_input_true: "constrains_an_input r \<Longrightarrow> cval (conjoin (\<lbrakk>\<rbrakk> r)) r ia = true"
-proof(induct r)
-  case (L x)
-  then show ?case by simp
-next
-  case (V x)
-  then show ?case
-    apply (case_tac x)
-    by (simp_all add: conjoin_def cval_And cval_true sorted_list_of_fset_def gval.simps)
-next
-  case (Plus r1 r2)
-  then show ?case
-    by (simp add: conjoin_def sorted_list_of_fset_def cval_And cval_true)
-next
-  case (Minus r1 r2)
-  then show ?case
-    by (simp add: conjoin_def sorted_list_of_fset_def cval_And cval_true)
-qed
-
-lemma consistent_posterior_gives_consistent_medial: "consistent (posterior c x) \<Longrightarrow> consistent (medial c (Guard x))"
-  apply (simp add: posterior_def Let_def posterior_separate_def)
-  apply (case_tac "consistent (medial c (Guard x))")
-   apply simp
-  by (simp add: inconsistent_false)
-
-lemma consistent_medial_gives_consistent_anterior: "consistent (medial c G) \<Longrightarrow> consistent c"
-  apply (simp add: consistent_def)
-  by (metis (full_types) fBall_funion medial_def)
-
-lemma transition_subsumes_self: "t \<^sub>c\<sqsupseteq> t"
+lemma transition_subsumes_self: "subsumes t c t"
   apply (simp add: subsumes_def)
-  apply (simp only: posterior_separate_def Let_def posterior_def medial_self_append)
-  apply (case_tac "consistent (medial c (Guard t))")
-   apply simp
-  by simp
-
-lemma medial_preserves_existing_elements: "x |\<in>| c r \<Longrightarrow> x |\<in>| medial c G r "
-  using anterior_subset_medial by blast
-
-lemma remove_obsolete_constraints_input: "remove_obsolete_constraints c s (V (I i)) = {|Bc True|}"
-  by (simp add: remove_obsolete_constraints_def)
-
-lemma filter_simp: "I i |\<notin>| fst |`| fset_of_list as \<Longrightarrow>
-(\<exists>n. aexp_constrains a (V (I n))) \<or> V aa = a \<or> fBex (fset_of_list as) (\<lambda>x. V (fst x) = a) =
-(\<exists>n. aexp_constrains a (V (I n))) \<or> fBex (fset_of_list as) (\<lambda>x. V (fst x) = a)"
   by auto
+
+primrec posterior_sequence :: "transition_matrix \<Rightarrow> cfstate \<Rightarrow> registers \<Rightarrow> trace \<Rightarrow> registers option" where
+  "posterior_sequence _ _ r [] = Some r" |
+  "posterior_sequence e s r (a#t) = (case step e s r (fst a) (snd a) of
+                                            None \<Rightarrow> None |
+                                            Some (_, s', _, r') \<Rightarrow> posterior_sequence e s' r' t
+                                         )"
+
+abbreviation anterior_context :: "transition_matrix \<Rightarrow> trace \<Rightarrow> registers option" where
+  "anterior_context e t \<equiv> posterior_sequence e 0 <> t"
+
+lemma posterior_sequence_accepts: "\<forall>s d. posterior_sequence e s d t = Some ca \<longrightarrow> accepts e s d t"
+proof(induct t)
+  case Nil
+  then show ?case
+    by (simp add: accepts.base)
+next
+  case (Cons a t)
+  then show ?case
+    apply clarify
+    apply simp
+     apply (case_tac "step e s d (fst a) (snd a)")
+     apply simp
+    apply (case_tac aa)
+    apply simp
+    apply (rule accepts.step)
+     apply simp
+    by simp
+qed
+
+lemma anterior_context_accepts: "\<exists>c. anterior_context e p = Some c \<Longrightarrow> accepts_trace e p"
+  using posterior_sequence_accepts
+  by auto
+
+lemma accepts_gives_context: "\<forall>s d. accepts e s d t \<longrightarrow> (\<exists>c. posterior_sequence e s d t = Some c)"
+proof(induct t)
+case Nil
+  then show ?case
+    by simp
+next
+  case (Cons a t)
+  then show ?case
+    apply clarify
+    apply simp
+     apply (case_tac "step e s d (fst a) (snd a)")
+     apply simp
+     apply (simp add: conditions_inaccepts)
+    apply simp
+    apply (case_tac aa)
+    apply simp
+    using inaccepts_future_inaccepts by blast
+qed
+
+lemma accepts_trace_gives_context: "accepts_trace e p \<Longrightarrow> (\<exists>c. anterior_context e p = Some c)"
+  using accepts_gives_context by auto
 
 end
